working on lts correctness

src/Pipit.System.fst
@@ -65,7 +65,225 @@ let rec system_of_exp (e: exp) (vars: nat) (#hwf: squash (wf e vars)):
     let (| st1, t1 |) = system_of_exp e1 (vars + 1) in
     (| st1, (fun (i: C.vector value vars) s s' r ->
       t1 (r :: i) s s' r) |)
-  
+
+let rec stepn
+  (#outer #vars: nat)
+  (#state: Type)
+  (e: exp)
+  (t: xsystem vars state)
+  (streams: C.table (outer + 1) vars)
+  (vs: C.vector value (outer + 1))
+  (s': state): prop =
+  match streams, vs with
+  | C.Table [C.Row row], [r] -> t row None s' r
+  | C.Table (C.Row row :: streams'), r :: vs' ->
+    exists (s'': state).
+      stepn #(outer - 1) e t (C.Table streams') vs' s'' /\
+      t row (Some s'') s' r
+
+let rec system_of_exp_invariant
+  (#outer #vars: nat)
+  (#state: Type)
+  (e: exp)
+  (t: xsystem vars state)
+  (#hwf: squash (wf e vars))
+  (#hsys: squash (system_of_exp e vars == (| state, t|)))
+  (streams: C.table (outer + 1) vars)
+  (vs: C.vector value (outer + 1))
+  (hBS: bigstep streams e vs)
+  (s: state):
+    Tot Type (decreases e) =
+  match e with
+  | XVar _ -> unit
+  | XVal _ -> unit
+  | XPrim2 _ e1 e2 ->
+    let (| st1, t1 |) = system_of_exp e1 vars in
+    let (| st2, t2 |) = system_of_exp e2 vars in
+    let (s1, s2) = s <: (st1 * st2) in
+    let BSPrim2 _ _ _ _ vs1 vs2 hBS1 hBS2 = hBS in
+    system_of_exp_invariant e1 t1 streams vs1 hBS1 s1 *
+    system_of_exp_invariant e2 t2 streams vs2 hBS2 s2
+  | XPre e1 ->
+    let BSPre _ _ _ vs1 hBS1 = hBS in
+    let (| st1, t1 |) = system_of_exp e1 vars in
+    let (s1, v) = s <: (st1 * value) in
+    (hBS': bigstep streams e1 (v :: vs1) * unit)
+      // & system_of_exp_invariant #outer #vars e1 t1 streams (v :: vs1) hBS' s1)
+
+  | XThen e1 e2 ->
+    let (| st1, t1 |) = system_of_exp e1 vars in
+    let (| st2, t2 |) = system_of_exp e2 vars in
+    let s2 = s <: st2 in
+    let BSThen _ _ _ vs1 vs2 hBS1 hBS2 = hBS in
+    system_of_exp_invariant e2 t2 streams vs2 hBS2 s2
+  | XMu e1 ->
+    let (| st1, t1 |) = system_of_exp e1 (vars + 1) in
+    let s1 = s <: st1 in
+    let BSMu _ _ vs1 hBS1 = hBS in
+    let hBS' = bigstep_substitute_XMu e1 streams vs hBS in
+    system_of_exp_invariant #outer #(vars + 1) e1 t1 (C.table_map_append (C.table_of_values vs1) streams) vs1 hBS' s1
+
+let rec step0_ok
+  (#vars: nat)
+  (#state: Type)
+  (e: exp { causal e })
+  (t: xsystem vars state)
+  (#hwf: squash (wf e vars))
+  (#hsys: squash (system_of_exp e vars == (| state, t|)))
+  (row: C.vector value vars)
+  (v: value)
+  (hBS: bigstep (C.Table [C.Row row]) e [v]):
+    (s': state & squash (t row None s' v) & system_of_exp_invariant #0 e t (C.Table [C.Row row]) [v] hBS s') =
+  match e with
+  | XVal _ ->
+    (| (), (), () |)
+
+  | XVar x ->
+    (| (), (), () |)
+
+  | XPrim2 p e1 e2 ->
+    let BSPrim2 _ _ _ _ [v1] [v2] hBS1 hBS2 = hBS in
+    let (| st1, t1 |) = system_of_exp e1 vars in
+    let (| st2, t2 |) = system_of_exp e2 vars in
+    let (| s1', _, ei1 |) = step0_ok e1 t1 row v1 hBS1 in
+    let (| s2', _, ei2 |) = step0_ok e2 t2 row v2 hBS2 in
+    (| (s1', s2'), (), (ei1, ei2) |)
+
+  | XPre e1 ->
+    begin
+    match hBS with
+    | BSPre _ _ _ [] hBS1 ->
+        let (| v1, hBS1' |) = bigstep_monotone_inv #0 #vars #(C.Table [C.Row row]) hBS1 in
+        let (| st1, t1 |) = system_of_exp e1 vars in
+        let (| s1', _, ei1 |) = step0_ok e1 t1 row v1 hBS1' in
+        let s' = (s1', v1) in
+        assert (
+          system_of_exp_invariant #0 #vars e t (C.Table #1 #vars [C.Row row]) [v] hBS s' ==
+          (hBS': bigstep (C.Table #1 #vars [C.Row row]) e1 [v1] * unit));
+          // (hBS': bigstep (C.Table [C.Row row]) e1 [v1] & system_of_exp_invariant #0 #vars e1 t1 (C.Table [C.Row row]) [v1] hBS' s1'));
+        let h': (hBS': bigstep (C.Table [C.Row row]) e1 [v1] & system_of_exp_invariant #0 #vars e1 t1 (C.Table [C.Row row]) [v1] hBS' s1') =
+          (| hBS1', ei1 |) in
+        let h'': system_of_exp_invariant #0 #vars e t _ [v] hBS s' =
+          ( hBS1', () ) in
+        (| s', (), h'' |)
+
+    | _ -> false_elim ()
+    end
+    // admit ()
+
+  // | XPre e1 ->
+  //   let BSPre _ _ _ [] hBS1 = hBS in
+  //   let (| v1, hBS1' |) = bigstep_monotone_inv hBS1 in
+  //   let (| st1, t1 |) = system_of_exp e1 vars in
+  //   let (| s1', _, ei1 |) = step0_ok e1 t1 row v1 hBS1' in
+  //   let streams = C.Table [C.Row row] in
+  //   let ei1' : system_of_exp_invariant #0 #vars e1 t1 streams [v1] hBS1' s1' = ei1 in
+  //   assert (v == xpre_init);
+  //   assert (system_of_exp_invariant #0 #vars (XPre e1) t streams [v] hBS (s1', v1) == (hBS': bigstep streams e1 [v1] & system_of_exp_invariant #0 #vars e1 t1 streams [v1] hBS' s1')) by (FStar.Tactics.compute (); FStar.Tactics.dump "ok");
+  //   let hb = (| hBS1', ei1' |) <: system_of_exp_invariant (XPre e1) t streams [v] hBS (s1', v1) in
+  //   (| (s1', v1), (), (| hBS1', ei1' |) |)
+
+  | _ -> admit ()
+
+
+let rec stepn_ok
+  (#outer #vars: nat)
+  (#state: Type)
+  (e: exp)
+  (t: xsystem vars state)
+  (#hwf: squash (wf e vars))
+  (#hsys: squash (system_of_exp e vars == (| state, t|)))
+  (streams: C.table (outer + 1) vars)
+  (vs: C.vector value (outer + 1))
+  (hBS: bigstep streams e vs):
+    (s': state & squash (stepn e t streams vs s')) =
+  match e, streams, vs with
+  | XVal _, C.Table [r], [v] ->
+    (| (), _ |)
+  | XVal _, C.Table (_ :: streams'), v :: vs' ->
+    let (| u, _ |) = stepn_ok #(outer - 1) e t (C.Table streams') vs' (bigstep_monotone hBS) in
+    (| u, _ |)
+
+  | XVar x, C.Table [r], [v] ->
+    (| (), _ |)
+  | XVar x, C.Table (_ :: streams'), v :: vs' ->
+    let (| u, _ |) = stepn_ok #(outer - 1) e t (C.Table streams') vs' (bigstep_monotone hBS) in (| u, _ |)
+  | XPrim2 p e1 e2, C.Table [r], [v] ->
+    let BSPrim2 _ _ _ _ [r1] [r2] hBS1 hBS2 = hBS in
+    let (| st1, t1 |) = system_of_exp e1 vars in
+    let (| st2, t2 |) = system_of_exp e2 vars in
+    let (| s1', _ |) = stepn_ok e1 t1 streams [r1] hBS1 in
+    let (| s2', _ |) = stepn_ok e2 t2 streams [r2] hBS2 in
+    (| (s1', s2'), _ |)
+
+  | XPrim2 p e1 e2, C.Table (C.Row row :: streams'), v :: vs' ->
+    let BSPrim2 _ _ _ _ vs1 vs2 hBS1 hBS2 = hBS in
+    let (| st1, t1 |) = system_of_exp e1 vars in
+    let (| st2, t2 |) = system_of_exp e2 vars in
+    let (| s, _ |) = stepn_ok #(outer - 1) e t (C.Table streams') vs' (bigstep_monotone hBS) in
+    let (s1, s2) = s <: (st1 * st2) in
+    let (| s1', _ |) = stepn_ok e1 t1 streams vs1 hBS1 in
+    let (| s2', _ |) = stepn_ok e2 t2 streams vs2 hBS2 in
+    assert (stepn #(outer - 1) e1 t1 (C.Table streams') (List.Tot.tl vs1) s1);
+    assert (v == eval_prim2 p (List.Tot.hd vs1) (List.Tot.hd vs2));
+    assert (stepn #(outer - 1) e t (C.Table streams') vs' (s1, s2));
+    assert (t1 row (Some s1) s1' (List.Tot.hd vs1));
+    assert (t2 row (Some s2) s2' (List.Tot.hd vs2));
+    assert (t row (Some s) (s1', s2') v);
+    assert (stepn e t streams vs (s1', s2'));
+    (| (s1', s2'), _ |)
+
+
+  // | XVar _, C.Table (_ :: streams'), v :: vs' -> (| (), _ |)
+  | _ -> admit ()
+  // match streams, vs with
+  // | C.Table [C.Row row], [r], [r'] ->
+  //   step0_ok e t row r r' s' hBS
+  // | C.Table (C.Row row :: streams'), r :: vs_e', r' :: vs_t' ->
+  //   admit ()
+    // eliminate exists (s_mid: state). stepn #(outer - 1) e t (C.Table streams') vs_t' s_mid
+    // returns vs_e == vs_t
+    // with hEx.
+    //   let hBS' = bigstep_monotone hBS in
+    //   let _ = stepn_ok #(outer - 1) e t (C.Table streams') vs_e' vs_t' s_mid hBS' in
+    //   match e with
+    //   | XVal _ -> ()
+    //   | XVar _ -> ()
+    //   | XPrim2 p e1 e2 ->
+    //     assert (vs_e' == vs_t');
+    //     let BSPrim2 _ _ _ _ vs_e1 vs_e2 hBS1 hBS2 = hBS in
+    //     let (| st1, t1 |) = system_of_exp e1 vars in
+    //     let (| st2, t2 |) = system_of_exp e2 vars in
+    //     let (s1, s2)   = s_mid <: (st1 * st2) in
+    //     let (s1', s2') = s' <: (st1 * st2) in
+    //     eliminate exists (r1' r2': value). t1 row (Some s1) s1' r1' /\ t2 row (Some s2) s2' r2' /\ r' == eval_prim2 p r1' r2'
+    //     returns r == r'
+    //     with hEx. begin
+    //          let _ = stepn_ok e1 t1 streams vs_e1 vs_e1 s1' hBS1 in
+    //          let _ = stepn_ok e2 t2 streams vs_e2 vs_e2 s2' hBS2 in
+    //          ()
+    //          end
+    //   | _ -> admit ()
+      //   | XPre e1 -> ()
+      //   | XThen e1 e2 ->
+      //   let BSThen _ _ _ [r1] [r2] hBS1 hBS2 = hBS in
+      //   let (| st1, t1 |) = system_of_exp e1 vars in
+      //   let (| st2, t2 |) = system_of_exp e2 vars in
+      //   eliminate exists (s1': st1) (r2': value). t1 row None s1' r' /\ t2 row None s' r2'
+      //   returns r == r'
+      //   with hEx. begin
+      //        let _ = step0_ok e1 t1 row r1 r' s1' hBS1 in
+      //        ()
+      //        end
+      //   | XMu e1 ->
+      //   let BSMu _ _ [r] hBS1 = hBS in
+      //   let (| st1, t1 |) = system_of_exp e1 (vars + 1) in
+      //   let hBS' = bigstep_recursive_XMu #0 e1 (C.table1 (C.Row row)) [] r r' hBS in
+      //   let _ = step0_ok e1 t1 (r' :: row) r r' s' hBS' in
+      //   ()
+
+
+
 let rec step0_ok
   (#vars: nat)
   (#state: Type)
@@ -74,11 +292,9 @@ let rec step0_ok
   (#hwf: squash (wf e vars))
   (#hsys: squash (system_of_exp e vars == (| state, t|)))
   (row: C.vector value vars)
-  (r r': value)
-  (s': state)
-  (hBS: bigstep (C.table1 (C.Row row)) e (C.vector1 r))
-  (#ht: squash (t row None s' r')):
-   Tot (squash (r == r')) (decreases e) =
+  (r: value)
+  (hBS: bigstep (C.table1 (C.Row row)) e (C.vector1 r)):
+   Tot (squash (exists (s': state). t row None s' r)) (decreases e) =
  match e with
  | XVal _ -> ()
  | XVar _ -> ()
@@ -86,28 +302,190 @@ let rec step0_ok
    let BSPrim2 _ _ _ _ [r1] [r2] hBS1 hBS2 = hBS in
    let (| st1, t1 |) = system_of_exp e1 vars in
    let (| st2, t2 |) = system_of_exp e2 vars in
-   let (s1', s2') = s' <: (st1 * st2) in
-   eliminate exists (r1' r2': value). t1 row None s1' r1' /\ t2 row None s2' r2' /\ r' == eval_prim2 p r1' r2'
-   returns r == r'
-   with hEx. begin
-     let _ = step0_ok e1 t1 row r1 r1' s1' hBS1 in
-     let _ = step0_ok e2 t2 row r2 r2' s2' hBS2 in
-     ()
-   end
- | XPre e1 -> ()
- | XThen e1 e2 ->
-   let BSThen _ _ _ [r1] [r2] hBS1 hBS2 = hBS in
-   let (| st1, t1 |) = system_of_exp e1 vars in
-   let (| st2, t2 |) = system_of_exp e2 vars in
-   eliminate exists (s1': st1) (r2': value). t1 row None s1' r' /\ t2 row None s' r2'
-   returns r == r'
-   with hEx. begin
-     let _ = step0_ok e1 t1 row r1 r' s1' hBS1 in
-     ()
-   end
- | XMu e1 ->
-   let BSMu _ _ [r] hBS1 = hBS in
-   let (| st1, t1 |) = system_of_exp e1 (vars + 1) in
-   let hBS' = bigstep_recursive_XMu #0 e1 (C.table1 (C.Row row)) [] r r' hBS in
-   let _ = step0_ok e1 t1 (r' :: row) r r' s' hBS' in
-   ()
+   let _ = step0_ok e1 t1 row r1 hBS1 in
+   let _ = step0_ok e2 t2 row r2 hBS2 in
+
+   eliminate exists (s1' : st1) (s2': st2). t1 row None s1' r1 /\ t2 row None s2' r2 /\ r == eval_prim2 p r1 r2
+   returns _ with hEx.
+     assert (t row None (s1', s2') r)
+
+ | XPre e1 ->
+    begin
+   match hBS with
+    | BSPre _ _ _ [] hBS1 ->
+        let (| st1, t1 |) = system_of_exp e1 vars in
+        let _ = step0_ok e1 t1 row r1 hBS1 in
+
+        eliminate exists (s1' : st1). t1 row None s1' r1 /\ r == true
+        returns _ with hEx.
+            assert (t row None s1' r)
+    // | _ -> admit () // false_elim ()
+    end
+ | _ -> admit ()
+ // | XPre e1 -> ()
+ // | XThen e1 e2 ->
+ //   let BSThen _ _ _ [r1] [r2] hBS1 hBS2 = hBS in
+ //   let (| st1, t1 |) = system_of_exp e1 vars in
+ //   let (| st2, t2 |) = system_of_exp e2 vars in
+ //   eliminate exists (s1': st1) (r2': value). t1 row None s1' r' /\ t2 row None s' r2'
+ //   returns r == r'
+ //   with hEx. begin
+ //     let _ = step0_ok e1 t1 row r1 r' s1' hBS1 in
+ //     ()
+ //   end
+ // | XMu e1 ->
+ //   let BSMu _ _ [r] hBS1 = hBS in
+ //   let (| st1, t1 |) = system_of_exp e1 (vars + 1) in
+ //   let hBS' = bigstep_recursive_XMu #0 e1 (C.table1 (C.Row row)) [] r r' hBS in
+ //   let _ = step0_ok e1 t1 (r' :: row) r r' s' hBS' in
+ //   ()
+
+// let rec stepn_ok
+//   (#outer #vars: nat)
+//   (#state: Type)
+//   (e: exp)
+//   (t: xsystem vars state)
+//   (#hwf: squash (wf e vars))
+//   (#hsys: squash (system_of_exp e vars == (| state, t|)))
+//   (streams: C.table (outer + 1) vars)
+//   (vs: C.vector value outer)
+//   (r r': value)
+//   (s': state)
+//   (hBS: bigstep streams e (r :: vs))
+//   (#ht: squash (stepn e t streams (r' :: vs) s')):
+//    Tot (squash (r == r')) =
+//   match streams with
+//   | C.Table [C.Row row] ->
+//     step0_ok e t row r r' s' hBS
+//   | C.Table (C.Row row :: streams') ->
+//     eliminate exists (s_mid: state). stepn #(outer - 1) e t (C.Table streams') vs s_mid
+//     returns r == r'
+//     with hEx.
+//       let hBS' = bigstep_monotone hBS in
+//       let _ = stepn_ok #(outer - 1) e t (C.Table streams') vs_e' vs_t' s_mid hBS' in
+//       match e with
+//       | XVal _ -> ()
+//       | XVar _ -> ()
+//       | XPrim2 p e1 e2 ->
+//         let BSPrim2 _ _ _ _ vs_e1 vs_e2 hBS1 hBS2 = hBS in
+//         let (| st1, t1 |) = system_of_exp e1 vars in
+//         let (| st2, t2 |) = system_of_exp e2 vars in
+//         let (s1, s2)   = s_mid <: (st1 * st2) in
+//         let (s1', s2') = s' <: (st1 * st2) in
+//         eliminate exists (r1' r2': value). t1 row (Some s1) s1' r1' /\ t2 row (Some s2) s2' r2' /\ r' == eval_prim2 p r1' r2'
+//         returns r == r'
+//         with hEx. begin
+//              let _ = stepn_ok e1 t1 streams () r1' s1' hBS1 in
+//              let _ = stepn_ok e2 t2 streams r2 r2' s2' hBS2 in
+//              ()
+//              end
+//       | _ -> admit ()
+//       //   | XPre e1 -> ()
+//       //   | XThen e1 e2 ->
+//       //   let BSThen _ _ _ [r1] [r2] hBS1 hBS2 = hBS in
+//       //   let (| st1, t1 |) = system_of_exp e1 vars in
+//       //   let (| st2, t2 |) = system_of_exp e2 vars in
+//       //   eliminate exists (s1': st1) (r2': value). t1 row None s1' r' /\ t2 row None s' r2'
+//       //   returns r == r'
+//       //   with hEx. begin
+//       //        let _ = step0_ok e1 t1 row r1 r' s1' hBS1 in
+//       //        ()
+//       //        end
+//       //   | XMu e1 ->
+//       //   let BSMu _ _ [r] hBS1 = hBS in
+//       //   let (| st1, t1 |) = system_of_exp e1 (vars + 1) in
+//       //   let hBS' = bigstep_recursive_XMu #0 e1 (C.table1 (C.Row row)) [] r r' hBS in
+//       //   let _ = step0_ok e1 t1 (r' :: row) r r' s' hBS' in
+//       //   ()
+
+let rec stepn_ok
+  (#outer #vars: nat)
+  (#state: Type)
+  (e: exp)
+  (t: xsystem vars state)
+  (#hwf: squash (wf e vars))
+  (#hsys: squash (system_of_exp e vars == (| state, t|)))
+  (streams: C.table (outer + 1) vars)
+  (vs_e vs_t: C.vector value (outer + 1))
+  (s': state)
+  (hBS: bigstep streams e vs_e)
+  (#ht: squash (stepn e t streams vs_t s')):
+   Tot (squash (vs_e == vs_t)) =
+  match streams, vs_e, vs_t with
+  | C.Table [C.Row row], [r], [r'] ->
+    step0_ok e t row r r' s' hBS
+  | C.Table (C.Row row :: streams'), r :: vs_e', r' :: vs_t' ->
+    eliminate exists (s_mid: state). stepn #(outer - 1) e t (C.Table streams') vs_t' s_mid
+    returns vs_e == vs_t
+    with hEx.
+      let hBS' = bigstep_monotone hBS in
+      let _ = stepn_ok #(outer - 1) e t (C.Table streams') vs_e' vs_t' s_mid hBS' in
+      match e with
+      | XVal _ -> ()
+      | XVar _ -> ()
+      | XPrim2 p e1 e2 ->
+        assert (vs_e' == vs_t');
+        let BSPrim2 _ _ _ _ vs_e1 vs_e2 hBS1 hBS2 = hBS in
+        let (| st1, t1 |) = system_of_exp e1 vars in
+        let (| st2, t2 |) = system_of_exp e2 vars in
+        let (s1, s2)   = s_mid <: (st1 * st2) in
+        let (s1', s2') = s' <: (st1 * st2) in
+        eliminate exists (r1' r2': value). t1 row (Some s1) s1' r1' /\ t2 row (Some s2) s2' r2' /\ r' == eval_prim2 p r1' r2'
+        returns r == r'
+        with hEx. begin
+             let _ = stepn_ok e1 t1 streams vs_e1 vs_e1 s1' hBS1 in
+             let _ = stepn_ok e2 t2 streams vs_e2 vs_e2 s2' hBS2 in
+             ()
+             end
+      | _ -> admit ()
+      //   | XPre e1 -> ()
+      //   | XThen e1 e2 ->
+      //   let BSThen _ _ _ [r1] [r2] hBS1 hBS2 = hBS in
+      //   let (| st1, t1 |) = system_of_exp e1 vars in
+      //   let (| st2, t2 |) = system_of_exp e2 vars in
+      //   eliminate exists (s1': st1) (r2': value). t1 row None s1' r' /\ t2 row None s' r2'
+      //   returns r == r'
+      //   with hEx. begin
+      //        let _ = step0_ok e1 t1 row r1 r' s1' hBS1 in
+      //        ()
+      //        end
+      //   | XMu e1 ->
+      //   let BSMu _ _ [r] hBS1 = hBS in
+      //   let (| st1, t1 |) = system_of_exp e1 (vars + 1) in
+      //   let hBS' = bigstep_recursive_XMu #0 e1 (C.table1 (C.Row row)) [] r r' hBS in
+      //   let _ = step0_ok e1 t1 (r' :: row) r r' s' hBS' in
+      //   ()
+
+
+ // match e with
+ // | XVal _ -> ()
+ // | XVar _ -> ()
+ // | XPrim2 p e1 e2 ->
+ //   let BSPrim2 _ _ _ _ [r1] [r2] hBS1 hBS2 = hBS in
+ //   let (| st1, t1 |) = system_of_exp e1 vars in
+ //   let (| st2, t2 |) = system_of_exp e2 vars in
+ //   let (s1', s2') = s' <: (st1 * st2) in
+ //   eliminate exists (r1' r2': value). t1 row None s1' r1' /\ t2 row None s2' r2' /\ r' == eval_prim2 p r1' r2'
+ //   returns r == r'
+ //   with hEx. begin
+ //     let _ = step0_ok e1 t1 row r1 r1' s1' hBS1 in
+ //     let _ = step0_ok e2 t2 row r2 r2' s2' hBS2 in
+ //     ()
+ //   end
+ // | XPre e1 -> ()
+ // | XThen e1 e2 ->
+ //   let BSThen _ _ _ [r1] [r2] hBS1 hBS2 = hBS in
+ //   let (| st1, t1 |) = system_of_exp e1 vars in
+ //   let (| st2, t2 |) = system_of_exp e2 vars in
+ //   eliminate exists (s1': st1) (r2': value). t1 row None s1' r' /\ t2 row None s' r2'
+ //   returns r == r'
+ //   with hEx. begin
+ //     let _ = step0_ok e1 t1 row r1 r' s1' hBS1 in
+ //     ()
+ //   end
+ // | XMu e1 ->
+ //   let BSMu _ _ [r] hBS1 = hBS in
+ //   let (| st1, t1 |) = system_of_exp e1 (vars + 1) in
+ //   let hBS' = bigstep_recursive_XMu #0 e1 (C.table1 (C.Row row)) [] r r' hBS in
+ //   let _ = step0_ok e1 t1 (r' :: row) r r' s' hBS' in
+ //   ()
